vyperMiscScript.sml
@@ -1,0 +1,297 @@
+Theory vyperMisc
+Ancestors
+  byte pair int_bitwise rich_list
+  cv_std vfmTypes
+Libs
+  cv_transLib blastLib
+
+(* Miscellaneous definitions/theorems/translations that need to be organised
+ * and upstreamed to HOL where appropriate *)
+
+Definition CHR_o_w2n_def:
+  CHR_o_w2n (b: byte) = CHR (w2n b)
+End
+
+val CHR_o_w2n_pre_def = cv_auto_trans_pre "CHR_o_w2n_pre" CHR_o_w2n_def;
+
+Theorem CHR_o_w2n_pre[cv_pre]:
+  CHR_o_w2n_pre x
+Proof
+  rw[CHR_o_w2n_pre_def]
+  \\ qspec_then`x`mp_tac wordsTheory.w2n_lt
+  \\ rw[]
+QED
+
+Theorem CHR_o_w2n_eq:
+  CHR_o_w2n = CHR o w2n
+Proof
+  rw[FUN_EQ_THM, CHR_o_w2n_def]
+QED
+
+Definition MAP_HEX_def:
+  MAP_HEX [] = [] ∧
+  MAP_HEX (x::xs) = HEX x :: MAP_HEX xs
+End
+
+val MAP_HEX_pre_def = cv_auto_trans_pre "MAP_HEX_pre" MAP_HEX_def;
+
+Theorem MAP_HEX_pre_EVERY:
+  MAP_HEX_pre ls = EVERY (λx. x < 16) ls
+Proof
+  Induct_on`ls` \\ rw[Once MAP_HEX_pre_def]
+QED
+
+Theorem MAP_HEX_MAP:
+  MAP_HEX = MAP HEX
+Proof
+  simp[FUN_EQ_THM]
+  \\ Induct \\ rw[MAP_HEX_def]
+QED
+
+val num_to_dec_string_pre_def =
+  ASCIInumbersTheory.num_to_dec_string_def
+  |> SRULE [ASCIInumbersTheory.n2s_def, FUN_EQ_THM, GSYM MAP_HEX_MAP]
+  |> cv_trans_pre "num_to_dec_string_pre";
+
+Theorem num_to_dec_string_pre[cv_pre]:
+  num_to_dec_string_pre x
+Proof
+  rw[num_to_dec_string_pre_def, MAP_HEX_pre_EVERY]
+  \\ qspecl_then[`10`,`x`]mp_tac numposrepTheory.n2l_BOUND
+  \\ rw[listTheory.EVERY_MEM]
+  \\ first_x_assum drule \\ rw[]
+QED
+
+Theorem int_exp_num:
+  (i:int) ** n =
+  if 0 ≤ i then &(Num i ** n)
+  else if EVEN n then &(Num (-i) ** n)
+  else -&(Num (-i) ** n)
+Proof
+  Cases_on`i` \\ simp[integerTheory.INT_POW_NEG]
+QED
+
+val () = cv_trans int_exp_num;
+
+Theorem Num_int_exp:
+  0 ≤ i ⇒ Num (i ** n) = Num i ** n
+Proof
+  Cases_on`i` \\ rw[]
+QED
+
+(* TODO: I don't know if this is the best way to translate this... *)
+val () = cv_auto_trans num_of_bits_def;
+val () = cv_auto_trans int_of_bits_def;
+val () = cv_auto_trans bits_of_int_def;
+
+Definition bits_bitwise_and_def:
+  bits_bitwise_and = bits_bitwise $/\
+End
+
+val bits_bitwise_and_pre_def = (bits_bitwise_def
+ |> oneline
+ |> Q.GEN`f`
+ |> Q.ISPEC`$/\`
+ |> SRULE [GSYM bits_bitwise_and_def]
+ |> cv_trans_pre_rec "bits_bitwise_and_pre")
+    (WF_REL_TAC `inv_image ($< LEX $<) (λ(x,y). (cv_size x, cv_size y))`
+     \\ rw[]
+     \\ Cases_on`cv_v` \\ gvs[]
+     \\ Cases_on`cv_v0` \\ gvs[]
+     \\ qmatch_assum_rename_tac`_ (cv_ispair p)`
+     \\ Cases_on`p` \\ gvs[]
+     \\ qmatch_assum_rename_tac`_ (cv_ispair p)`
+     \\ Cases_on`p` \\ gvs[]);
+
+Theorem bits_bitwise_and_pre[cv_pre]:
+  ∀x y. bits_bitwise_and_pre x y
+Proof
+  simp[FORALL_PROD]
+  \\ qid_spec_tac`f:bool -> bool -> bool`
+  \\ ho_match_mp_tac bits_bitwise_ind
+  \\ rw[]
+  \\ rw[Once bits_bitwise_and_pre_def]
+QED
+
+val () = int_and_def
+  |> SRULE [FUN_EQ_THM, int_bitwise_def, GSYM bits_bitwise_and_def]
+  |> cv_trans;
+
+Definition bits_bitwise_or_def:
+  bits_bitwise_or = bits_bitwise $\/
+End
+
+val bits_bitwise_or_pre_def = (bits_bitwise_def
+ |> oneline
+ |> Q.GEN`f`
+ |> Q.ISPEC`$\/`
+ |> SRULE [GSYM bits_bitwise_or_def]
+ |> cv_trans_pre_rec "bits_bitwise_or_pre")
+    (WF_REL_TAC `inv_image ($< LEX $<) (λ(x,y). (cv_size x, cv_size y))`
+     \\ rw[]
+     \\ Cases_on`cv_v` \\ gvs[]
+     \\ Cases_on`cv_v0` \\ gvs[]
+     \\ qmatch_assum_rename_tac`_ (cv_ispair p)`
+     \\ Cases_on`p` \\ gvs[]
+     \\ qmatch_assum_rename_tac`_ (cv_ispair p)`
+     \\ Cases_on`p` \\ gvs[]);
+
+Theorem bits_bitwise_or_pre[cv_pre]:
+  ∀x y. bits_bitwise_or_pre x y
+Proof
+  simp[FORALL_PROD]
+  \\ qid_spec_tac`f:bool -> bool -> bool`
+  \\ ho_match_mp_tac bits_bitwise_ind
+  \\ rw[]
+  \\ rw[Once bits_bitwise_or_pre_def]
+QED
+
+val () = int_or_def
+  |> SRULE [FUN_EQ_THM, int_bitwise_def, GSYM bits_bitwise_or_def]
+  |> cv_trans;
+
+Definition bits_bitwise_xor_def:
+  bits_bitwise_xor = bits_bitwise ((≠) : bool -> bool -> bool)
+End
+
+val bits_bitwise_xor_pre_def = (bits_bitwise_def
+ |> oneline
+ |> Q.GEN`f`
+ |> Q.ISPEC`λx:bool y. x ≠ y`
+ |> SRULE [GSYM bits_bitwise_xor_def]
+ |> cv_trans_pre_rec "bits_bitwise_xor_pre")
+    (WF_REL_TAC `inv_image ($< LEX $<) (λ(x,y). (cv_size x, cv_size y))`
+     \\ rw[]
+     \\ Cases_on`cv_v` \\ gvs[]
+     \\ Cases_on`cv_v0` \\ gvs[]
+     \\ qmatch_assum_rename_tac`_ (cv_ispair p)`
+     \\ Cases_on`p` \\ gvs[]
+     \\ qmatch_assum_rename_tac`_ (cv_ispair p)`
+     \\ Cases_on`p` \\ gvs[]);
+
+Theorem bits_bitwise_xor_pre[cv_pre]:
+  ∀x y. bits_bitwise_xor_pre x y
+Proof
+  simp[FORALL_PROD]
+  \\ qid_spec_tac`f:bool -> bool -> bool`
+  \\ ho_match_mp_tac bits_bitwise_ind
+  \\ rw[]
+  \\ rw[Once bits_bitwise_xor_pre_def]
+QED
+
+val () = int_xor_def
+  |> SRULE [FUN_EQ_THM, int_bitwise_def, GSYM bits_bitwise_xor_def]
+  |> cv_trans;
+
+val () = cv_auto_trans int_shift_left_def;
+val () = cv_auto_trans int_shift_right_def;
+
+Theorem set_byte_160:
+  set_byte a b (w: 160 word) be =
+  let i = byte_index a be in
+       if i =   0 then w2w b        || w && 0xFFFFFFFFFFFFFFFFFFFFFFFFFFFFFFFFFFFFFF00w
+  else if i =   8 then w2w b <<   8 || w && 0xFFFFFFFFFFFFFFFFFFFFFFFFFFFFFFFFFFFF00FFw
+  else if i =  16 then w2w b <<  16 || w && 0xFFFFFFFFFFFFFFFFFFFFFFFFFFFFFFFFFF00FFFFw
+  else if i =  24 then w2w b <<  24 || w && 0xFFFFFFFFFFFFFFFFFFFFFFFFFFFFFFFF00FFFFFFw
+  else if i =  32 then w2w b <<  32 || w && 0xFFFFFFFFFFFFFFFFFFFFFFFFFFFFFF00FFFFFFFFw
+  else if i =  40 then w2w b <<  40 || w && 0xFFFFFFFFFFFFFFFFFFFFFFFFFFFF00FFFFFFFFFFw
+  else if i =  48 then w2w b <<  48 || w && 0xFFFFFFFFFFFFFFFFFFFFFFFFFF00FFFFFFFFFFFFw
+  else if i =  56 then w2w b <<  56 || w && 0xFFFFFFFFFFFFFFFFFFFFFFFF00FFFFFFFFFFFFFFw
+  else if i =  64 then w2w b <<  64 || w && 0xFFFFFFFFFFFFFFFFFFFFFF00FFFFFFFFFFFFFFFFw
+  else if i =  72 then w2w b <<  72 || w && 0xFFFFFFFFFFFFFFFFFFFF00FFFFFFFFFFFFFFFFFFw
+  else if i =  80 then w2w b <<  80 || w && 0xFFFFFFFFFFFFFFFFFF00FFFFFFFFFFFFFFFFFFFFw
+  else if i =  88 then w2w b <<  88 || w && 0xFFFFFFFFFFFFFFFF00FFFFFFFFFFFFFFFFFFFFFFw
+  else if i =  96 then w2w b <<  96 || w && 0xFFFFFFFFFFFFFF00FFFFFFFFFFFFFFFFFFFFFFFFw
+  else if i = 104 then w2w b << 104 || w && 0xFFFFFFFFFFFF00FFFFFFFFFFFFFFFFFFFFFFFFFFw
+  else if i = 112 then w2w b << 112 || w && 0xFFFFFFFFFF00FFFFFFFFFFFFFFFFFFFFFFFFFFFFw
+  else if i = 120 then w2w b << 120 || w && 0xFFFFFFFF00FFFFFFFFFFFFFFFFFFFFFFFFFFFFFFw
+  else if i = 128 then w2w b << 128 || w && 0xFFFFFF00FFFFFFFFFFFFFFFFFFFFFFFFFFFFFFFFw
+  else if i = 136 then w2w b << 136 || w && 0xFFFF00FFFFFFFFFFFFFFFFFFFFFFFFFFFFFFFFFFw
+  else if i = 144 then w2w b << 144 || w && 0xFF00FFFFFFFFFFFFFFFFFFFFFFFFFFFFFFFFFFFFw
+  else if i = 152 then w2w b << 152 || w && 0x00FFFFFFFFFFFFFFFFFFFFFFFFFFFFFFFFFFFFFFw
+  else                 w2w b << 160 || w && 0xFFFFFFFFFFFFFFFFFFFFFFFFFFFFFFFFFFFFFFFFw
+Proof
+  rw_tac std_ss [set_byte_def, word_slice_alt_def]
+  \\ reverse(rpt IF_CASES_TAC)
+  >- (
+    `i = 160`
+    by (
+      qunabbrev_tac`i`
+      \\ full_simp_tac (std_ss ++ boolSimps.LET_ss ++ ARITH_ss) [
+            byte_index_def, EVAL``dimindex(:160)``]
+      \\ `w2n a MOD 20 < 20` by rw[]
+      \\ pop_assum mp_tac
+      \\ qmatch_goalsub_abbrev_tac`z < 20 ⇒ f`
+      \\ simp_tac std_ss [wordsTheory.NUMERAL_LESS_THM]
+      \\ strip_tac \\ gs[Abbr`f`]
+      \\ rw[] \\ gs[] )
+    \\ asm_simp_tac std_ss []
+    \\ simp_tac (srw_ss()) []
+    \\ BBLAST_TAC)
+  \\ asm_simp_tac std_ss []
+  \\ simp_tac (srw_ss()) []
+  \\ BBLAST_TAC
+QED
+
+val () = cv_auto_trans set_byte_160;
+
+val () = cv_auto_trans (INST_TYPE [alpha |-> “:160”] word_of_bytes_def);
+
+Theorem SUM_MAP_FILTER_MEM_LE:
+  MEM x ls /\ ~P x ==>
+  SUM (MAP f (FILTER P ls)) + f x <= SUM (MAP f ls)
+Proof
+  qid_spec_tac`x`
+  \\ Induct_on`ls`
+  \\ rw[] \\ gs[]
+  >- (
+    irule SUM_SUBLIST \\ simp[]
+    \\ irule MAP_SUBLIST \\ simp[]
+    \\ irule FILTER_sublist )
+  \\ first_x_assum drule \\ rw[]
+QED
+
+Theorem list_size_SUM_MAP:
+  list_size f ls = LENGTH ls + SUM (MAP f ls)
+Proof
+  Induct_on `ls` \\ rw[listTheory.list_size_def]
+QED
+
+Theorem list_size_pair_size_map:
+  list_size (pair_size f1 f2) ls =
+  list_size f1 (MAP FST ls) +
+  list_size f2 (MAP SND ls)
+Proof
+  Induct_on`ls` \\ rw[]
+  \\ Cases_on`h` \\ gvs[]
+QED
+
+Definition member_def:
+  member x [] = F ∧
+  member x (y::ys) = ((x = y) ∨ member x ys)
+End
+
+val () = cv_trans member_def;
+
+Theorem member_intro:
+  ∀x ys. MEM x ys = member x ys
+Proof
+  Induct_on `ys` \\ rw[member_def]
+QED
+
+Theorem cv_size_cv_map_snd_le:
+  ∀l. cv_size (cv_map_snd l) ≤ cv_size l
+Proof
+  ho_match_mp_tac cv_map_snd_ind
+  \\ rw[]
+  \\ rw[Once cv_map_snd_def] \\ gvs[]
+  \\ Cases_on`l` \\ gvs[]
+  \\ qmatch_goalsub_rename_tac`cv_snd p`
+  \\ Cases_on`p` \\ gvs[]
+QED
+
+Definition string_to_num_def:
+  string_to_num s = l2n 257 (MAP (SUC o ORD) s)
+End
+
+val () = cv_auto_trans string_to_num_def;
