vyperSmallStepScript.sml
@@ -1,7 +1,7 @@
 Theory vyperSmallStep
 Ancestors
   arithmetic combin pair list while
-  vyperInterpreter
+  vyperMisc vyperInterpreter
 Libs
   cv_transLib
 
@@ -529,7 +529,7 @@ Definition apply_val_def:
   apply_val cx v2 st (SubscriptK1 tv1 k) =
     liftk cx ApplyTv (do
       ts <- lift_option (get_self_code cx) "Subscript get_self_code";
-      lift_sum (evaluate_subscript ts tv1 v2)
+      lift_sum (evaluate_subscript (type_env ts) tv1 v2)
     od st) k ∧
   apply_val cx v st (AttributeK id k) =
     liftk cx (ApplyTv o Value) (lift_sum (evaluate_attribute v id) st) k ∧
