README.md
@@ -52,6 +52,10 @@ This theory defines functions for re-running execution traces, as used in the Vy
 
 The decoding of JSON into our AST type is somewhat ad-hoc, in part because the JSON format is not fully specified. In future work, we might formalise more of the front-end or elaboration process, including parsing and type-checking, so that we can run source code directly. For now, we rely on an external front-end (e.g., as used in Vyper's test export process) and decode its output to construct terms in our formal syntax.
 
+### vyperMisc
+
+Some helper functions and theorems, some of which might eventually be upstreamed to the HOL repository.
+
 ## What is Missing
 
 The focus of this work so far has been the core execution semantics of Vyper contract code, as abstract syntax, for external calls into a single contract. Therefore, the main limitations are _calls to other contracts_ (and other chain interaction like deploying contracts during execution), and _elaboration into abstract syntax_ done by the Vyper compiler front-end. Our intention is to remove all these limitations in future work to build a comprehensive and definitive formal semantics for the entire Vyper language.
